src/program_proof/tulip/paxos/program/paxos.v
@@ -96,18 +96,20 @@ Section repr.
                     then own_paxos_candidate_only nid termc terml termp entsc entspP resppP nids γ
                     else True).
 
-  Definition own_paxos_leader_only (termc : u64) (ents : list string) γ : iProp Σ :=
-    ∃ (entsbase : list string),
-      "Hps"   ∷ own_proposal γ (uint.nat termc) ents ∗
-      "#Hpsb" ∷ is_base_proposal_receipt γ (uint.nat termc) entsbase ∗
-      "%Hpsb" ∷ ⌜prefix entsbase ents⌝.
+  Definition own_paxos_leader_only
+    (termc : u64) (log : list string) (lsnpeersP : loc) γ : iProp Σ :=
+    ∃ (lsnpeers : gmap u64 u64),
+      "Hps"        ∷ own_proposal γ (uint.nat termc) log ∗
+      "Hlsnpeers"  ∷ own_map lsnpeersP (DfracOwn 1) lsnpeers ∗
+      "#Hpfb"      ∷ prefix_base_ledger γ (uint.nat termc) log ∗
+      "%Hlelenlog" ∷ ⌜map_Forall (λ _ i, (uint.nat i ≤ length log)%nat) lsnpeers⌝.
 
   Definition own_paxos_leader
-    (paxos : loc) (termc : u64) (ents : list string) (isleader : bool) γ : iProp Σ :=
+    (paxos : loc) (termc : u64) (log : list string) (isleader : bool) γ : iProp Σ :=
     ∃ (lsnpeersP : loc),
       "HisleaderP" ∷ paxos ↦[Paxos :: "isleader"] #isleader ∗
       "HlsnpeersP" ∷ paxos ↦[Paxos :: "lsnpeers"] #lsnpeersP ∗
-      "Honlyl"     ∷ (if isleader then own_paxos_leader_only termc ents γ else True).
+      "Honlyl"     ∷ (if isleader then own_paxos_leader_only termc log lsnpeersP γ else True).
 
   Definition own_paxos_sc (paxos : loc) (nids : gset u64) : iProp Σ :=
     ∃ (sc : u64),
@@ -173,6 +175,11 @@ Section repr.
     (paxos : loc) (nidme termc : u64) nids γ : iProp Σ :=
     ∃ (terml lsnc : u64),
       own_paxos_internal paxos nidme termc terml lsnc false false nids γ.
+
+  Definition own_paxos_leading_with_termc
+    (paxos : loc) (nidme termc : u64) nids γ : iProp Σ :=
+    ∃ (terml lsnc : u64) (iscand : bool),
+      own_paxos_internal paxos nidme termc terml lsnc iscand true nids γ.
 
   Definition own_paxos_with_termc_terml
     (paxos : loc) (nidme termc terml : u64) nids γ : iProp Σ :=
@@ -838,9 +845,13 @@ Section ascend.
     (*@     // Transit from the candidate to the leader.                        @*)
     (*@     px.iscand = false                                                   @*)
     (*@     px.isleader = true                                                  @*)
+    (*@     px.lsnpeers = make(map[uint64]uint64)                               @*)
     (*@                                                                         @*)
-    iNamed "Hleader". iNamed "Honlyl".
+    iNamed "Hleader".
     do 2 wp_storeField.
+    wp_apply (wp_NewMap u64 u64).
+    iIntros (lsnpeersP') "Hlsnpeers".
+    wp_storeField.
 
     (*@     // Logical action: Ascend(@px.termc, @px.log).                      @*)
     (*@                                                                         @*)
@@ -865,7 +876,7 @@ Section ascend.
     set log' := logc ++ entsp.
     set logc' := take (uint.nat lsnc) log'.
     iAssert (own_paxos_leader px termc log' true γ)%I
-      with "[$HisleaderP $HlsnpeersP $Hps]" as "Hleader".
+      with "[$HisleaderP $HlsnpeersP $Hlsnpeers $Hps]" as "Hleader".
     { by iFrame "Hpsb". }
     iDestruct (safe_ledger_above_mono (uint.nat terml) logc' (uint.nat termc) with "[]")
       as "Hcmted'".
@@ -1216,6 +1227,89 @@ Section accept.
   Qed.
 
 End accept.
+
+Section obtain.
+  Context `{!heapGS Σ, !paxos_ghostG Σ}.
+
+  Theorem wp_Paxos__obtain (px : loc) (nid : u64) (nidme termc : u64) nids γ :
+    {{{ own_paxos_leading_with_termc px nidme termc nids γ }}}
+      Paxos__obtain #px #nid
+    {{{ (lsne : u64) (entsP : Slice.t) (ents loga : list string), RET (#lsne, (to_val entsP)); 
+        own_paxos_leading_with_termc px nidme termc nids γ ∗
+        own_slice entsP stringT (DfracOwn 1) ents ∗
+        prefix_base_ledger γ (uint.nat termc) loga ∗
+        prefix_growing_ledger γ (uint.nat termc) loga ∗
+        ⌜drop (uint.nat lsne) loga = ents⌝
+    }}}.
+  Proof.
+    iIntros (Φ) "Hpx HΦ".
+    wp_rec.
+
+    (*@ func (px *Paxos) obtain(nid uint64) (uint64, []string) {                @*)
+    (*@     lsne, ok := px.lsnpeers[nid]                                        @*)
+    (*@                                                                         @*)
+    iNamed "Hpx". iNamed "Hleader". iNamed "Honlyl".
+    wp_loadField.
+    wp_apply (wp_MapGet with "Hlsnpeers").
+    iIntros (lsne ok) "[%Hok Hlsnpeers]".
+    wp_pures.
+
+    (*@     if !ok {                                                            @*)
+    (*@         // The follower has not reported the matched LSN, so send an    @*)
+    (*@         // empty APPEND-ENTRIES request.                                @*)
+    (*@         return uint64(len(px.log)), make([]string, 0)                   @*)
+    (*@     }                                                                   @*)
+    (*@                                                                         @*)
+    iAssert (prefix_growing_ledger γ (uint.nat termc) log)%I as "#Hpfg".
+    { iDestruct (proposal_witness with "Hps") as "#Hpslb".
+      by iFrame "Hpslb".
+    }
+    iNamed "Hpx".
+    iDestruct (own_slice_sz with "Hlog") as %Hszlog.
+    wp_if_destruct.
+    { wp_loadField.
+      wp_apply wp_slice_len.
+      wp_apply wp_NewSlice.
+      iIntros (entsP) "Hents".
+      wp_pures.
+      iApply "HΦ".
+      iFrame "Hcand".
+      iFrame "∗ # %".
+      iPureIntro.
+      by rewrite -Hszlog drop_all uint_nat_W64_0 /=.
+    }
+    apply map_get_true in Hok.
+    apply Hlelenlog in Hok.
+
+    (*@     // The follower has reported up to where the log is matched         @*)
+    (*@     // (i.e., @lsne), so send everything after that.                    @*)
+    (*@     ents := make([]string, uint64(len(px.log)) - lsne)                  @*)
+    (*@     copy(ents, px.log[lsne :])                                          @*)
+    (*@                                                                         @*)
+    wp_loadField.
+    wp_apply wp_slice_len.
+    wp_apply wp_NewSlice.
+    iIntros (entsP) "Hents".
+    iDestruct (own_slice_sz with "Hents") as %Hszents.
+    wp_loadField.
+    iDestruct (own_slice_small_acc with "Hlog") as "[Hlog HlogC]".
+    iDestruct (own_slice_small_acc with "Hents") as "[Hents HentsC]".
+    wp_apply (wp_SliceCopy_SliceSkip_src with "[$Hlog $Hents]").
+    { clear -Hok. word. }
+    { rewrite length_replicate. clear -Hszents Hszlog Hok. word. }
+    iIntros "[Hlog Hents]".
+    iDestruct ("HlogC" with "Hlog") as "Hlog".
+    iDestruct ("HentsC" with "Hents") as "Hents".
+    wp_pures.
+
+    (*@     return lsne, ents                                                   @*)
+    (*@ }                                                                       @*)
+    iApply "HΦ".
+    iFrame "Hcand".
+    by iFrame "∗ # %".
+  Qed.
+
+End obtain.
 
 Section program.
   Context `{!heapGS Σ, !paxos_ghostG Σ}.
